theories/Substitution/Introductions/Pi.v
@@ -18,6 +18,46 @@ Proof.
   bsimpl ; now substify.
 Qed. *)
 
+Section PolyRedPi.
+  Context `{GenericTypingProperties}.
+
+  Lemma LRPiPoly0 {Γ l A B} (PAB : PolyRed Γ l A B) : [Γ ||-Π<l> tProd A B].
+  Proof.
+    econstructor; tea; pose proof (polyRedId PAB) as []; escape.
+    + eapply redtywf_refl; gen_typing.
+    + eapply convty_prod; tea; unshelve eapply escapeEq; tea; eapply LRTyEqRefl_.
+  Defined.
+
+  Definition LRPiPoly {Γ l A B} (PAB : PolyRed Γ l A B) : [Γ ||-<l> tProd A B] := LRPi' (LRPiPoly0 PAB).
+
+  Lemma LRPiPolyEq0 {Γ l A A' B B'} (PAB : PolyRed Γ l A B) (Peq : PolyRedEq PAB A' B') :
+    [Γ |- A'] -> [Γ ,, A' |- B'] ->
+    [Γ ||-Π tProd A B ≅ tProd A' B' | LRPiPoly0 PAB].
+  Proof.
+    econstructor; cbn; tea.
+    + eapply redtywf_refl; gen_typing.
+    + pose proof (polyRedEqId PAB Peq) as []; escape.
+      eapply convty_prod; tea.
+      eapply escape; now apply (polyRedId PAB).
+  Qed.
+
+  Lemma LRPiPolyEq {Γ l A A' B B'} (PAB : PolyRed Γ l A B) (Peq : PolyRedEq PAB A' B') :
+    [Γ |- A'] -> [Γ ,, A' |- B'] ->
+    [Γ ||-<l> tProd A B ≅ tProd A' B' | LRPiPoly PAB].
+  Proof.
+    now eapply LRPiPolyEq0.
+  Qed.
+
+  Lemma LRPiPolyEq' {Γ l A A' B B'} (PAB : PolyRed Γ l A B) (Peq : PolyRedEq PAB A' B') (RAB : [Γ ||-<l> tProd A B]):
+    [Γ |- A'] -> [Γ ,, A' |- B'] ->
+    [Γ ||-<l> tProd A B ≅ tProd A' B' | RAB].
+  Proof.
+    intros; irrelevanceRefl; now eapply LRPiPolyEq.
+  Qed.
+  
+End PolyRedPi.
+
+
 Section PiTyValidity.
 
   Context `{GenericTypingProperties}.
